lib/falcon/bv32_falcon_lemmas.i.dfy
@@ -1,0 +1,300 @@
+include "../../arch/riscv/machine.s.dfy"
+include "../../arch/riscv/vale.i.dfy"
+include "ntt_model.dfy"
+include "../bv32_ops.dfy"
+
+include "../DivModNeg.dfy"
+
+module bv32_falcon_lemmas {
+    import opened Seq
+    import opened Power
+    import opened Power2
+    import opened DivMod
+    import opened Mul
+    import opened DivModNeg
+    import opened integers
+    import opened bv32_ops
+    import opened rv_machine
+    import opened rv_vale
+    import opened mem
+
+    import opened ntt_model
+    import opened nth_root
+    import opened pows_of_2
+  	import opened ntt_polys
+
+    predicate fvar_iter_inv(heap: heap_t, iter: b16_iter, address: int, index: int)
+    {
+        && b16_iter_inv(iter, heap, if address >= 0 then address else iter.cur_ptr())
+        && (index >= 0 ==> iter.index == index)
+        && |iter.buff| == N.full
+        && buff_is_nsized(iter.buff)
+    }
+
+    predicate {:opaque} buff_is_nsized(a: seq<uint16>)
+    {
+      && (|a| == N.full)
+      && (forall i | 0 <= i < N.full :: a[i] < Q)
+    }
+
+    function {:opaque} buff_as_nsized(a: seq<uint16>): (a': n_sized)
+      requires buff_is_nsized(a);
+      ensures a == a';
+    {
+      reveal buff_is_nsized();
+      a
+    }
+
+    function lsize(view: loop_view): (r: pow2_t)
+        requires view.loop_view_wf();
+        ensures r.full <= N.full
+    {
+        assume view.hsize.full <= N.full;
+        view.lsize()
+    }
+
+    predicate s_loop_inv(a: seq<uint16>, hcount: pow2_t, j: nat, bi: nat, view: loop_view)
+    {
+        && buff_is_nsized(a)
+        && view.s_loop_inv(buff_as_nsized(a), hcount, j, bi)
+    }
+
+    lemma s_loop_inv_pre_lemma(
+        a: seq<uint16>,
+        p: seq<uint16>,
+        hcount: pow2_t,
+        j: nat,
+        t: pow2_t,
+        s5: uint32,
+        view: loop_view)
+
+        requires N == pow2_t_cons(9, 512);
+        requires j_loop_inv(a, hcount, j, view);
+        requires t == lsize(view);
+        requires j < lsize(view).full;
+        requires t.full < BASE_32;
+        requires s5 == uint32_ls(uint32_add(t.full, j), 1);
+
+        ensures s_loop_inv(a, hcount, j, 0, view);
+    {
+        view.s_loop_inv_pre_lemma(buff_as_nsized(a), hcount, j);
+        rev_mixed_powers_mont_table_lemma(t, hcount, j);
+
+        assert uint32_add(t.full, j) == t.full + j;
+
+    }
+
+    predicate s_loop_update(a: seq<uint16>, a': seq<uint16>, hcount: pow2_t, j: nat, bi: nat, view: loop_view)
+        requires s_loop_inv(a, hcount, j, bi, view);
+        requires bi < hcount.full
+    {
+        && buff_is_nsized(a')
+        && view.s_loop_update(buff_as_nsized(a), buff_as_nsized(a'), hcount, j, bi)
+    }
+
+    lemma s_loop_inv_peri_lemma(a: seq<uint16>, a': seq<uint16>, hcount: pow2_t, j: nat, bi: nat, view: loop_view)
+        requires s_loop_inv(a, hcount, j, bi, view);
+        requires bi < hcount.full
+        requires s_loop_update(a, a', hcount, j, bi, view);
+        ensures s_loop_inv(a', hcount, j, bi+1, view);
+    {
+        view.s_loop_inv_peri_lemma(a, a', hcount, j, bi);
+    }
+
+    lemma higher_points_view_index_lemma(a: seq<uint16>, hcount: pow2_t, j: nat, bi: nat, view: loop_view)
+        returns (s: nat)
+    
+        requires s_loop_inv(a, hcount, j, bi, view);
+        requires bi < hcount.full
+        ensures s == bi + (2*j) * hcount.full;
+        ensures s + hcount.full < N.full;
+        ensures a[s] ==
+            level_points_view(buff_as_nsized(a), view.hsize)[bi][2*j];
+        ensures s == point_view_index(bi, 2*j, view.hsize);
+        ensures a[s+hcount.full] ==
+            level_points_view(buff_as_nsized(a), view.hsize)[bi][2*j+1];
+        ensures s+hcount.full == point_view_index(bi, 2*j+1, view.hsize);
+    {
+        s := view. higher_points_view_index_lemma(buff_as_nsized(a), hcount, j, bi);
+    }
+
+    predicate t_loop_inv(a: seq<uint16>, hcount: pow2_t, view: loop_view)
+    {
+      && buff_is_nsized(a)
+      && view.t_loop_inv(buff_as_nsized(a), hcount)
+    }
+
+    predicate j_loop_inv(a: seq<uint16>, hcount: pow2_t, j: nat, view: loop_view)
+    {
+        && buff_is_nsized(a)
+        && view.j_loop_inv(buff_as_nsized(a), hcount, j)
+    }
+
+    lemma j_loop_inv_pre_lemma(a: seq<uint16>, hcount: pow2_t, view: loop_view)
+        requires t_loop_inv(a, hcount, view);
+        ensures j_loop_inv(a, hcount, 0, view);
+    {
+        view.j_loop_inv_pre_lemma(buff_as_nsized(a), hcount);
+    }
+
+    lemma j_loop_inv_post_lemma(a: seq<uint16>, hcount: pow2_t, j: nat, view: loop_view)
+        returns (v': loop_view)
+    
+        requires j_loop_inv(a, hcount, j, view);
+        requires j == lsize(view).full;
+        requires 0 <= view.hsize.exp <= N.exp;
+
+        ensures v' == view.next_t_loop_view(hcount);
+        ensures view.hsize.exp < N.exp ==> t_loop_inv(a, pow2_half(hcount), v');
+        ensures view.hsize.exp == N.exp ==> t_loop_end(a, v');
+    {
+        v' := view.j_loop_inv_post_lemma(a, hcount, j);
+    }
+
+    predicate t_loop_end(a: seq<uint16>, view: loop_view)
+    {
+        && buff_is_nsized(a)
+        && view.t_loop_end(buff_as_nsized(a))
+    }
+
+    lemma lemma_rs_by_31(x: int32)
+      ensures x >= 0 ==> int32_rs(x, 31) == 0;
+      ensures x < 0 ==> int32_rs(x, 31) == -1;
+    {
+      assert integers.BASE_31 == Power2.Pow2(31) by { Power2.Lemma2To64(); }
+
+      if x >= 0 {
+        assert x / Power2.Pow2(31) == 0 by {
+          DivMod.LemmaBasicDivAuto();
+        }
+      } else {
+        assert x / Power2.Pow2(31) == -1 by {
+          DivModNeg.LemmaDivBounded(x, integers.BASE_31);
+        }
+      }
+    }
+
+
+    lemma lemma_mq_add_correct(d: uint32, b: uint32, c: uint32, r: uint32, x: int, y: int)
+        requires 0 <= x < 12289;
+        requires 0 <= y < 12289;
+        requires d == uint32_add(to_uint32(x), uint32_add(to_uint32(y), to_uint32((-12289))));
+        requires b == to_uint32(int32_rs(to_int32(d), 31));
+        requires c == uint32_and(b, to_uint32(12289));
+        requires r == uint32_add(c, d);
+        ensures r == (x + y) % 12289;
+    {
+      var Q : int := 12289;
+
+      // d == x + y - Q
+      assert IsModEquivalent(d, x + y - Q, BASE_32);
+
+      // -Q <= d < Q
+      assert 0 <= x + y < 2*Q;
+      assert (-Q) <= x + y - Q < Q;
+      assert (-Q) <= to_int32(d) < Q;
+
+      if to_int32(d) >= 0 {
+        assert int32_rs(to_int32(d), 31) == 0 by { lemma_rs_by_31(to_int32(d)); }
+        assert uint32_and(0, Q) == 0 by { reveal_and(); }
+        assert IsModEquivalent(r, x + y, Q);
+      }
+      else {
+        assert int32_rs(to_int32(d), 31) == -1 by { lemma_rs_by_31(to_int32(d)); }
+        assert uint32_and(b, Q) == Q by { reveal_and(); }
+        assert IsModEquivalent(r, x + y, Q);
+      }
+
+    } 
+
+    lemma lemma_mq_sub_correct(d: uint32, b: uint32, c: uint32, r: uint32, x: int, y: int)
+        requires 0 <= x < 12289;
+        requires 0 <= y < 12289;
+        requires d == uint32_sub(to_uint32(x), to_uint32(y));
+        requires b == to_uint32(int32_rs(to_int32(d), 31));
+        requires c == uint32_and(b, to_uint32(12289));
+        requires r == uint32_add(c, d);
+        ensures r == (x - y) % 12289;
+    {
+      var Q : int := 12289;
+      
+      assert IsModEquivalent(d, x - y, BASE_32);
+      assert -Q <= to_int32(d) < 2 * Q;
+      
+      if to_int32(d) >= 0 {
+        assert int32_rs(to_int32(d), 31) == 0 by { lemma_rs_by_31(to_int32(d)); }
+        assert uint32_and(b, Q) == 0 by { reveal_and(); }
+        assert IsModEquivalent(r, x - y, Q);
+      }
+      else {
+        assert int32_rs(to_int32(d), 31) == -1 by { lemma_rs_by_31(to_int32(d)); }
+        assert uint32_and(b, Q) == Q by { reveal_and(); }
+        assert IsModEquivalent(r, x - y, Q);
+      }
+    }
+
+    lemma lemma_positive_rs(x: uint32, shift: nat)
+      requires x >= 0;
+      requires x < BASE_31;
+      ensures to_uint32(int32_rs(x, shift)) == int32_rs(x, shift)
+    {
+      assert to_int32(x) == x;
+      assert int32_rs(to_int32(x), shift) >= 0 by { DivMod.LemmaDivBasicsAuto(); }
+    }
+
+     lemma lemma_mq_rshift1_correct(par: uint32, b: uint32, c: uint32, d: uint32, r: uint32, x: int)
+         requires 0 <= x < 12289;
+         requires par == uint32_and(x, 1);
+         requires b == uint32_sub(0, par);
+         requires c == uint32_and(b, 12289);
+         requires d == uint32_add(x, c);
+         requires r == to_uint32(int32_rs(to_int32(d), 1));
+ 
+         //ensures r == (x / 2) % 12289;
+         ensures IsModEquivalent(2 * r, x, 12289);
+         ensures r < 12289;
+     {
+       var Q : int := 12289;
+       assert par == 0 || par == 1 by { reveal_and(); }
+ 
+       if par == 0 {
+         assert b == 0;
+         assert c == 0 by { reveal_and(); }
+         assert x % 2 == 0 by { reveal_and(); }
+         assert d == x;
+         
+         assert 0 <= to_int32(d) < Q;
+         assert r == int32_rs(to_int32(d), 1) by { lemma_positive_rs(x, 1); }
+ 
+         assert r == d / Power2.Pow2(1);
+         assert r == d / 2 by { Power2.Lemma2To64(); }
+ 
+         assert IsModEquivalent(r, x / 2, Q);
+         
+       } else {
+         assert b == 0xffff_ffff;
+         assert c == Q by { reveal_and(); }
+         assert d == uint32_add(x, Q);
+         assert d == x + Q;
+
+         assert 0 <= to_int32(d) <= x + Q;
+         assert r == int32_rs(to_int32(d), 1) by { lemma_positive_rs(x + Q, 1); }
+ 
+         assert IsModEquivalent(d, x, Q);
+ 
+         assert r == d / Power2.Pow2(1);
+         assert r == d / 2 by { Power2.Lemma2To64(); }
+ 
+         assert r == (x + Q) / 2;
+         
+        //  assert x % 2 == 1 by { reveal_and(); }
+        assume x % 2 == 1;
+         assert Q % 2 == 1;
+         assert (x + Q) % 2 == 0 by { DivMod.LemmaModAdds(x, Q, 2); }
+ 
+         assert r == (x + Q) / 2;
+         assert IsModEquivalent(2 * r, x + Q, Q);
+       }
+     }
+
+}
